Combined sort_fg_client and sort_fg

theories/examples/sort_fg.v
@@ -2,7 +2,7 @@ From stdpp Require Export sorting.
 From actris.channel Require Import proto_channel proofmode.
 From iris.heap_lang Require Import proofmode notation.
 From iris.heap_lang Require Import assert.
-From actris.utils Require Import compare.
+From actris.utils Require Import llist compare.
 
 Definition cont := true.
 Definition stop := false.
@@ -50,6 +50,23 @@ Definition sort_service_fg : val :=
 Definition sort_service_fg_func : val := λ: "c",
   let: "cmp" := recv "c" in
   sort_service_fg "cmp" "c".
+
+Definition send_all : val :=
+  rec: "go" "c" "xs" :=
+    if: lisnil "xs" then #() else
+    send "c" #cont;; send "c" (lpop "xs");; "go" "c" "xs".
+
+Definition recv_all : val :=
+  rec: "go" "c" "ys" :=
+    if: ~recv "c" then #() else
+    let: "x" := recv "c" in
+    "go" "c" "ys";; lcons "x" "ys".
+
+Definition sort_client_fg : val := λ: "cmp" "xs",
+  let: "c" := start_chan (λ: "c", sort_service_fg "cmp" "c") in
+  send_all "c" "xs";;
+  send "c" #stop;;
+  recv_all "c" "xs".
 
 Section sort_fg.
   Context `{!heapG Σ, !proto_chanG Σ}.
@@ -220,6 +237,57 @@ Section sort_fg.
         wp_select. by iApply "HΨ".
     - wp_select. by iApply "HΨ".
   Qed.
+  
+  Lemma send_all_spec c p xs' l xs :
+    {{{ llist I l xs ∗ c ↣ (sort_fg_head_protocol xs' <++> p) }}}
+      send_all c #l
+    {{{ RET #(); llist I l [] ∗ c ↣ (sort_fg_head_protocol (xs' ++ xs) <++> p) }}}.
+  Proof.
+    iIntros (Φ) "[Hl Hc] HΦ".
+    iInduction xs as [|x xs] "IH" forall (xs').
+    { wp_lam. wp_apply (lisnil_spec with "Hl"); iIntros "Hl"; wp_pures.
+      iApply "HΦ". rewrite right_id_L. iFrame. }
+    wp_lam. wp_apply (lisnil_spec with "Hl"); iIntros "Hl". wp_select.
+    wp_apply (lpop_spec with "Hl"); iIntros (v) "[HIx Hl]".
+    wp_send with "[$HIx]". wp_apply ("IH" with "Hl Hc"). by rewrite -assoc_L.
+  Qed.
+
+  Lemma recv_all_spec c p l xs ys' :
+    Sorted R ys' →
+    {{{ llist I l [] ∗ c ↣ (sort_fg_tail_protocol xs ys' <++> p) }}}
+      recv_all c #l
+    {{{ ys, RET #();
+        ⌜Sorted R (ys' ++ ys)⌝ ∗ ⌜ys' ++ ys ≡ₚ xs⌝ ∗ llist I l ys ∗ c ↣ p
+    }}}.
+  Proof.
+    iIntros (Hsort Φ) "[Hl Hc] HΦ".
+    iLöb as "IH" forall (xs ys' Φ Hsort).
+    wp_lam. wp_branch as %_ | %Hperm; wp_pures.
+    - wp_recv (y v) as (Htl) "HIx".
+      wp_apply ("IH" with "[] Hl Hc"); first by auto using Sorted_snoc.
+      iIntros (ys). rewrite -!assoc_L. iDestruct 1 as (??) "[Hl Hc]".
+      wp_apply (lcons_spec with "[$Hl $HIx]"); iIntros "Hl"; wp_pures.
+      iApply ("HΦ" with "[$Hl $Hc]"); simpl; eauto.
+    - iApply ("HΦ" $! []); rewrite /= right_id_L; by iFrame.
+  Qed.
+
+  Lemma sort_client_fg_spec cmp l xs :
+    cmp_spec I R cmp -∗
+    {{{ llist I l xs }}}
+      sort_client_fg cmp #l
+    {{{ ys, RET #(); ⌜Sorted R ys⌝ ∗ ⌜ys ≡ₚ xs⌝ ∗ llist I l ys }}}.
+  Proof.
+    iIntros "#Hcmp !>" (Φ) "Hl HΦ". wp_lam.
+    wp_apply (start_chan_proto_spec (sort_fg_protocol <++> END)%proto);
+      iIntros (c) "Hc".
+    { wp_apply (sort_service_fg_spec with "Hcmp Hc"); auto. }
+    wp_apply (send_all_spec with "[$Hl $Hc]"); iIntros "[Hl Hc]".
+    wp_select.
+    wp_apply (recv_all_spec with "[$Hl $Hc]"); auto.
+    iIntros (ys) "/=". iDestruct 1 as (??) "[Hk _]".
+    iApply "HΦ"; auto with iFrame.
+  Qed.
+  
   End sort_fg_inner.
 
   Definition sort_fg_func_protocol : iProto Σ :=
